Foundation/Modal/Kripke/Preservation.lean
@@ -1,27 +1,32 @@
-import Foundation.Modal.Kripke.Semantics
-import Foundation.Logic.Kripke.Preservation
+import Foundation.Modal.Kripke.Closure
 
 
-namespace LO
+namespace LO.Modal
 
 namespace Kripke
 
-abbrev IrreflexiveFrameClass : FrameClass := { F | Irreflexive F }
-
-end Kripke
+open Formula.Kripke
 
 
-open LO.Kripke
+section Bisimulation
 
-namespace Modal.Kripke
+structure Model.Bisimulation (M₁ M₂ : Kripke.Model) where
+  toRel : Rel M₁.World M₂.World
+  atomic {x₁ : M₁.World} {x₂ : M₂.World} {a : ℕ} : toRel x₁ x₂ → ((M₁ x₁ a) ↔ (M₂ x₂ a))
+  forth {x₁ y₁ : M₁.World} {x₂ : M₂.World} : toRel x₁ x₂ → x₁ ≺ y₁ → ∃ y₂ : M₂.World, toRel y₁ y₂ ∧ x₂ ≺ y₂
+  back {x₁ : M₁.World} {x₂ y₂ : M₂.World} : toRel x₁ x₂ → x₂ ≺ y₂ → ∃ y₁ : M₁.World, toRel y₁ y₂ ∧ x₁ ≺ y₁
 
-open Formula
+infix:80 " ⇄ " => Model.Bisimulation
 
-def ModalEquivalent {M₁ M₂ : Kripke.Model α} (w₁ : M₁.World) (w₂ : M₂.World) : Prop := ∀ {φ}, w₁ ⊧ φ ↔ w₂ ⊧ φ
+instance : CoeFun (Model.Bisimulation M₁ M₂) (λ _ => M₁.World → M₂.World → Prop) := ⟨λ bi => bi.toRel⟩
+
+end Bisimulation
+
+
+section ModalEquivalent
+
+def ModalEquivalent {M₁ M₂ : Model} (w₁ : M₁.World) (w₂ : M₂.World) : Prop := ∀ {φ}, w₁ ⊧ φ ↔ w₂ ⊧ φ
 infix:50 " ↭ " => ModalEquivalent
-
-variable {F₁ F₂ : Kripke.Frame}
-         {M₁ M₂ : Kripke.Model α}
 
 lemma modal_equivalent_of_bisimilar (Bi : M₁ ⇄ M₂) (bisx : Bi x₁ x₂) : x₁ ↭ x₂ := by
   intro φ;
@@ -43,60 +48,320 @@ lemma modal_equivalent_of_bisimilar (Bi : M₁ ⇄ M₂) (bisx : Bi x₁ x₂) :
       exact ih bisy |>.mpr (h _ rx₂y₂);
   | _ => simp_all;
 
+end ModalEquivalent
 
-lemma modal_equivalence_of_modal_morphism (f : M₁ →ₚ M₂) (w : M₁.World) : w ↭ (f w) := by
+
+section PseudoEpimorphism
+
+structure Frame.PseudoEpimorphism (F₁ F₂ : Kripke.Frame) where
+  toFun : F₁.World → F₂.World
+  forth {x y : F₁.World} : x ≺ y → toFun x ≺ toFun y
+  back {w : F₁.World} {v : F₂.World} : toFun w ≺ v → ∃ u, toFun u = v ∧ w ≺ u
+
+infix:80 " →ₚ " => Frame.PseudoEpimorphism
+
+instance : CoeFun (Frame.PseudoEpimorphism F₁ F₂) (λ _ => F₁.World → F₂.World) := ⟨λ f => f.toFun⟩
+
+namespace Frame.PseudoEpimorphism
+
+variable {F F₁ F₂ F₃ : Kripke.Frame}
+
+def id : F →ₚ F where
+  toFun := _root_.id
+  forth := by simp;
+  back := by simp;
+
+def TransitiveClosure (f : F₁ →ₚ F₂) (F₂_trans : Transitive F₂) : F₁^+ →ₚ F₂ where
+  toFun := f.toFun
+  forth := by
+    intro x y hxy; simp at x y;
+    induction hxy with
+    | single hxy => exact f.forth hxy;
+    | @tail z y _ Rzy Rxz =>
+      replace Rzy := f.forth Rzy;
+      exact F₂_trans Rxz Rzy;
+  back := by
+    intro x w hxw;
+    obtain ⟨u, ⟨rfl, hxu⟩⟩ := f.back hxw;
+    use u;
+    constructor;
+    . rfl;
+    . exact Frame.RelTransGen.single hxu;
+
+def comp (f : F₁ →ₚ F₂) (g : F₂ →ₚ F₃) : F₁ →ₚ F₃ where
+  toFun := g ∘ f
+  forth := by
+    intro x y hxy;
+    exact g.forth $ f.forth hxy;
+  back := by
+    intro x w hxw;
+    simp at hxw;
+    obtain ⟨y, ⟨hyz, hxy⟩⟩ := g.back hxw;
+    obtain ⟨u, ⟨hgu, hfu⟩⟩ := f.back hxy;
+    use u;
+    constructor;
+    . subst_vars; simp;
+    . assumption;
+
+end Frame.PseudoEpimorphism
+
+
+structure Model.PseudoEpimorphism (M₁ M₂ : Kripke.Model) extends M₁.toFrame →ₚ M₂.toFrame where
+  atomic {w : M₁.World} : (M₁ w a) ↔ (M₂ (toFun w) a)
+
+infix:80 " →ₚ " => Model.PseudoEpimorphism
+
+instance : CoeFun (Model.PseudoEpimorphism M₁ M₂) (λ _ => M₁.World → M₂.World) := ⟨λ f => f.toFun⟩
+
+namespace Model.PseudoEpimorphism
+
+variable {M M₁ M₂ M₃ : Kripke.Model}
+
+def id : M →ₚ M where
+  toFun := _root_.id
+  forth := by simp;
+  back := by simp;
+  atomic := by simp;
+
+def mkAtomic (f : M₁.toFrame →ₚ M₂.toFrame) (atomic : ∀ {w a}, (M₁ w a) ↔ (M₂ (f w) a)) : M₁ →ₚ M₂ := {
+  toFun := f,
+  forth := f.forth,
+  back := f.back,
+  atomic := atomic,
+}
+
+def comp (f : M₁ →ₚ M₂) (g : M₂ →ₚ M₃) : M₁ →ₚ M₃ := mkAtomic (f.toPseudoEpimorphism.comp (g.toPseudoEpimorphism)) $ by
+  intro x φ;
+  constructor;
+  . intro h;
+    apply g.atomic.mp;
+    apply f.atomic.mp;
+    assumption;
+  . intro h;
+    apply f.atomic.mpr;
+    apply g.atomic.mpr;
+    assumption;
+
+def bisimulation (f : M₁ →ₚ M₂) : M₁ ⇄ M₂ := {
+  toRel := Function.graph f,
+  atomic := by
+    intro x₁ x₂ a e; subst e;
+    constructor;
+    . apply f.atomic.mp;
+    . apply f.atomic.mpr;
+  forth := by
+    simp;
+    intro x₁ y₁ rx₁y₁;
+    exact f.forth rx₁y₁;
+  back := by
+    simp;
+    intro x₁ x₂ y₂ e rx₂y₂; subst e;
+    obtain ⟨y₁, _⟩ := f.back rx₂y₂;
+    use y₁;
+}
+
+lemma modal_equivalence (f : M₁ →ₚ M₂) (w : M₁.World) : w ↭ (f w) := by
   apply modal_equivalent_of_bisimilar $ Model.PseudoEpimorphism.bisimulation f;
   simp [Model.PseudoEpimorphism.bisimulation];
 
-lemma iff_formula_valid_on_frame_surjective_morphism (f : F₁ →ₚ F₂) (f_surjective : Function.Surjective f) : F₁#α ⊧ φ → F₂#α ⊧ φ := by
+end Model.PseudoEpimorphism
+
+
+variable {F₁ F₂ : Kripke.Frame} {M₁ M₂ : Kripke.Model}
+
+lemma iff_formula_valid_on_frame_surjective_morphism (f : F₁ →ₚ F₂) (f_surjective : Function.Surjective f) : F₁ ⊧ φ → F₂ ⊧ φ := by
   contrapose;
   intro h;
-  obtain ⟨V₂, w₂, h⟩ := by simpa [Kripke.ValidOnFrame, Kripke.ValidOnModel] using h;
-  simp [Kripke.ValidOnFrame, Kripke.ValidOnModel];
+  obtain ⟨V₂, w₂, h⟩ := by simpa [ValidOnFrame, ValidOnModel] using h;
+  simp [ValidOnFrame, ValidOnModel];
 
   obtain ⟨w₁, e⟩ := f_surjective w₂; subst e;
   let V₁ := λ w a => V₂ (f w) a;
   use V₁, w₁;
 
-  let M₁ : Model α := { Frame := F₁, Valuation := V₁ };
-  let M₂ : Model α := { Frame := F₂, Valuation := V₂ };
-  exact modal_equivalence_of_modal_morphism (M₁ := M₁) (M₂ := M₂) {
+  exact Model.PseudoEpimorphism.modal_equivalence (M₁ := ⟨F₁, V₁⟩) (M₂ := ⟨F₂, V₂⟩) {
     toFun := f,
     forth := f.forth,
     back := f.back,
     atomic := by simp_all
   } w₁ |>.not.mpr h;
 
-lemma iff_theory_valid_on_frame_surjective_morphism (f : F₁ →ₚ F₂) (f_surjective : Function.Surjective f) : F₁#α ⊧* T → F₂#α ⊧* T := by
+lemma iff_theory_valid_on_frame_surjective_morphism (f : F₁ →ₚ F₂) (f_surjective : Function.Surjective f) : F₁ ⊧* T → F₂ ⊧* T := by
   simp only [Semantics.realizeSet_iff];
   intro h φ hp;
   exact iff_formula_valid_on_frame_surjective_morphism f f_surjective (h hp);
 
-theorem undefinable_irreflexive : ¬∃ (H : Hilbert α), ∀ F, F ∈ 𝔽(H) ↔ F ∈ IrreflexiveFrameClass.{0} := by
+end PseudoEpimorphism
+
+
+def Frame.isRooted (F : Frame) (r : F.World) : Prop := ∀ w ≠ r, r ≺ w
+
+structure RootedFrame extends Kripke.Frame where
+  root : World
+  root_rooted : Frame.isRooted _ root
+  default := root
+
+
+section PointGenerated
+
+def Frame.PointGenerated (F : Kripke.Frame) (r : F.World) : Kripke.RootedFrame where
+  World := { w | w = r ∨ r ≺ w }
+  Rel x y := x.1 ≺ y.1
+  world_nonempty := ⟨r, by tauto⟩
+  root := ⟨r, by tauto⟩
+  root_rooted := by
+    rintro ⟨x, (rfl | hx)⟩;
+    . intro h; contradiction;
+    . intro _; exact hx;
+infix:100 "↾" => Frame.PointGenerated
+
+namespace Frame.PointGenerated
+
+variable {F : Kripke.Frame} {r : F.World}
+
+lemma rel_transitive (F_trans : Transitive F) : Transitive (F↾r).Rel := by
+  rintro ⟨x, (rfl | hx)⟩ ⟨y, (rfl | hy)⟩ ⟨z, (rfl | hz)⟩ hxy hyz;
+  all_goals aesop;
+
+lemma rel_irreflexive (F_irrefl : Irreflexive F) : Irreflexive (F↾r).Rel := by
+  rintro ⟨x, (rfl | hx)⟩ h;
+  all_goals aesop;
+
+lemma rel_universal (F_refl : Reflexive F) (F_eucl : Euclidean F) : Universal (F↾r).Rel := by
+  have F_symm := symm_of_refl_eucl F_refl F_eucl;
+  rintro ⟨x, (rfl | hx)⟩ ⟨y, (rfl | hy)⟩;
+  . apply F_refl;
+  . exact hy;
+  . exact F_symm hx;
+  . apply F_symm $ F_eucl hx hy;
+
+instance [Finite F.World] : Finite (F↾r).World := by
+  simp [Frame.PointGenerated];
+  apply Subtype.finite;
+
+instance [DecidableEq F.World] : DecidableEq (F↾r).World := by
+  apply Subtype.instDecidableEq (p := λ w => w = r ∨ r ≺ w);
+
+end Frame.PointGenerated
+
+
+structure RootedModel extends Kripke.Model, Kripke.RootedFrame where
+
+
+def Model.PointGenerated (M : Kripke.Model) (r : M.World) : Kripke.RootedModel :=
+  letI rF := M.toFrame↾r;
+  {
+    toFrame := rF.toFrame
+    Val := λ w a => M.Val w.1 a
+    root := rF |>.root
+    root_rooted := rF.root_rooted
+  }
+infix:100 "↾" => Model.PointGenerated
+
+namespace Model.PointGenerated
+
+variable {M : Kripke.Model}
+
+def bisimulation_of_trans (M_trans : Transitive M.Rel) (r : M.World) : (M↾r).toModel ⇄ M where
+  toRel x y := x.1 = y
+  atomic := by
+    rintro x y a rfl;
+    simp [Model.PointGenerated];
+  forth := by
+    rintro x₁ y₁ x₂ rfl Rx₂y₁;
+    use y₁.1;
+    constructor;
+    . simp;
+    . exact Rx₂y₁;
+  back := by
+    rintro ⟨x₁, (rfl | hx₁)⟩ x₂ y₂ rfl Rx₂y₂;
+    . use ⟨y₂, by right; exact Rx₂y₂⟩;
+      constructor;
+      . simp;
+      . exact Rx₂y₂;
+    . use ⟨y₂, ?h₂⟩;
+      constructor;
+      . simp;
+      . exact Rx₂y₂;
+      right;
+      exact M_trans hx₁ Rx₂y₂;
+
+lemma modal_equivalent_at_root (M_trans : Transitive M.toFrame) (r : M.World) : ModalEquivalent (M₁ := (M↾r).toModel) (M₂ := M) ⟨r, by simp⟩ r
+  := modal_equivalent_of_bisimilar (bisimulation_of_trans M_trans r) $ by simp [bisimulation_of_trans];
+
+end Model.PointGenerated
+
+end PointGenerated
+
+
+section Generation
+
+structure Frame.GeneratedSub (F₁ F₂ : Kripke.Frame) extends F₁ →ₚ F₂ where
+ monic : Function.Injective toFun
+
+infix:80 " ⊆ₚ " => Frame.GeneratedSub
+
+end Generation
+
+
+/-
+namespace Frame
+
+variable {F : Kripke.Frame} (x : F.World)
+
+def successors := { w | x ≺^* w }
+postfix:100 "↑*" => Frame.upward
+
+def immediate_successors := { w | x ≺ w }
+postfix:100 "↑¹" => Frame.immediate_successor
+
+def proper_immediate_successors := { w | x ≠ w ∧ x ≺ w }
+postfix:100 "↑" => Frame.proper_immediate_successor
+
+
+def predeccsors := { w | w ≺^* x }
+postfix:100 "↓*" => Frame.downward
+
+def immediate_predeccsors := { w | w ≺ x }
+postfix:100 "↓¹" => Frame.immediate_predeccsor
+
+def proper_immediate_predeccsors := { w | w ≠ x ∧ w ≺ x }
+postfix:100 "↓" => Frame.proper_immediate_predeccsors
+
+end Frame
+-/
+
+
+abbrev IrreflexiveFrameClass : FrameClass := { F | Irreflexive F }
+
+theorem undefinable_irreflexive : ¬∃ Ax : Theory ℕ, IrreflexiveFrameClass.DefinedBy Ax := by
   by_contra hC;
   obtain ⟨Ax, h⟩ := hC;
 
-  let F₁ : Frame := { World := PUnit ⊕ PUnit, Rel := (· ≠ ·) };
-  have hIF₁ : Irreflexive F₁ := by simp [Irreflexive, Frame.Rel'];
-
-  let F₂ : Frame := { World := PUnit, Rel := (· = ·) };
+  let F₁ : Frame := { World := Fin 2, Rel := (· ≠ ·) };
+  let F₂ : Frame := { World := Fin 1, Rel := (· = ·) };
 
   let f : F₁ →ₚ F₂ := {
-    toFun := λ _ => (),
+    toFun := λ _ => 0,
     forth := by simp [Frame.Rel'],
-    back := by simp_all [Frame.Rel'];
+    back := by
+      simp [Frame.Rel'];
+      intro x;
+      use 1 - x;
+      omega;
   };
-  have f_surjective : Function.Surjective f := by simp [Function.Surjective];
+  have f_surjective : Function.Surjective f := by
+    simp [Function.Surjective];
+    aesop;
 
+  have : Irreflexive F₂ := by
+    apply h F₂ |>.mpr;
+    apply iff_theory_valid_on_frame_surjective_morphism f f_surjective;
+    exact h F₁ |>.mp $ by simp [Irreflexive, Frame.Rel'];
   have : ¬Irreflexive F₂ := by simp [Irreflexive];
-  have : Irreflexive F₂ := by simpa using
-    (h F₂ |>.mp $ (iff_theory_valid_on_frame_surjective_morphism f f_surjective ) (h F₁ |>.mpr hIF₁));
   contradiction;
 
-lemma modal_equivalent_at_root_on_generated_model
-  (M : Model α) (M_trans : Transitive M.Frame) (r : M.World) : ModalEquivalent (M₁ := M↾r) (M₂ := M) ⟨r, by simp⟩ r
-  := modal_equivalent_of_bisimilar (Model.PointGenerated.bisimulation M M_trans r) Model.PointGenerated.bisimulation.rooted
 
-end Modal.Kripke
+end Kripke
 
-end LO
+end LO.Modal
