Foundation/Modal/Kripke/Tree.lean
@@ -1,39 +1,20 @@
-import Mathlib.Data.Fintype.List
-import Foundation.Logic.Kripke.Preservation
+import Foundation.Vorspiel.Chain
+import Foundation.Modal.Kripke.Preservation
 
-namespace List
+namespace LO.Modal
 
-variable {l l₁ l₂ : List α}
-variable {R : α → α → Prop}
+namespace Kripke
 
-lemma Chain'.nodup_of_trans_irreflex (R_trans : Transitive R) (R_irrefl : Irreflexive R) (h_chain : l.Chain' R) : l.Nodup := by
-  by_contra hC;
-  replace ⟨d, hC⟩ := List.exists_duplicate_iff_not_nodup.mpr hC;
-  have := List.duplicate_iff_sublist.mp hC;
-  have := @List.Chain'.sublist α R [d, d] l ⟨by aesop⟩ h_chain this;
-  simp at this;
-  exact R_irrefl d this;
+open Relation (TransGen)
 
-instance finiteNodupList [DecidableEq α] [Finite α] : Finite { l : List α // l.Nodup } := @fintypeNodupList α _ (Fintype.ofFinite α) |>.finite
-
-lemma chains_finite [DecidableEq α] [Finite α] (R_trans : Transitive R) (R_irrefl : Irreflexive R) : Finite { l : List α // l.Chain' R } := by
-  apply @Finite.of_injective { l : List α // l.Chain' R } { l : List α // l.Nodup } _ ?f;
-  case f => intro ⟨l, hl⟩; refine ⟨l, List.Chain'.nodup_of_trans_irreflex R_trans R_irrefl hl⟩;
-  simp [Function.Injective];
-
-end List
-
-
-namespace LO.Kripke
+variable {F : Frame} {r : F.World}
 
 def Frame.TreeUnravelling (F : Frame) (r : F.World) : Kripke.Frame where
   World := { c : List F.World | [r] <+: c ∧ c.Chain' F.Rel }
-  World_nonempty := ⟨[r], (by simp)⟩
   Rel cx cy := ∃ z, cx.1 ++ [z] = cy.1
+  world_nonempty := ⟨[r], (by simp)⟩
 
 namespace Frame.TreeUnravelling
-
-variable {F : Frame} {r : F.World}
 
 @[simp]
 lemma not_nil {c : (F.TreeUnravelling r).World} : c.1 ≠ [] := by
@@ -87,10 +68,6 @@ end Frame.TreeUnravelling
 abbrev Frame.TransitiveTreeUnravelling (F : Frame) (r : F.World) := (F.TreeUnravelling r)^+
 
 namespace Frame.TransitiveTreeUnravelling
-
-open Relation (TransGen)
-
-variable {F : Frame} {r : F.World}
 
 @[simp]
 lemma not_nil {c : (F.TransitiveTreeUnravelling r).World} : c.1 ≠ [] := by
@@ -168,28 +145,32 @@ def pMorphism (F : Frame) (F_trans : Transitive F.Rel) (r : F) : (F.TransitiveTr
 end Frame.TransitiveTreeUnravelling
 
 
-def Model.TreeUnravelling (M : Kripke.Model α) (r : M.World) : Kripke.Model α where
-  Frame := M.Frame.TreeUnravelling r
-  Valuation c a := M.Valuation (c.1.getLast (by simp)) a
+def Model.TreeUnravelling (M : Kripke.Model) (r : M.World) : Kripke.Model where
+  toFrame := M.toFrame.TreeUnravelling r
+  Val c a := M.Val (c.1.getLast (by simp)) a
 
 namespace Model.TreeUnravelling
 
-variable {M : Kripke.Model α} {r : M.World}
+variable {M : Kripke.Model} {r : M.World}
 
-def pMorphism (M : Kripke.Model α) (r : M.World) : M.TreeUnravelling r →ₚ M :=
-  Model.PseudoEpimorphism.mkAtomic (Frame.TreeUnravelling.PMorphism M.Frame r) $ by aesop;
+def pMorphism (M : Kripke.Model) (r : M.World) : M.TreeUnravelling r →ₚ M :=
+  Model.PseudoEpimorphism.mkAtomic (Frame.TreeUnravelling.PMorphism M.toFrame r) $ by aesop;
 
 end Model.TreeUnravelling
 
 
-def Model.TransitiveTreeUnravelling (M : Kripke.Model α) (r : M.World) : Kripke.Model α where
-  Frame := M.Frame.TransitiveTreeUnravelling r
-  Valuation c a := M.Valuation (c.1.getLast (by simp)) a
+def Model.TransitiveTreeUnravelling (M : Kripke.Model) (r : M.World) : Kripke.Model where
+  toFrame := M.toFrame.TransitiveTreeUnravelling r
+  Val c a := M.Val (c.1.getLast (by simp)) a
 
 namespace Model.TransitiveTreeUnravelling
 
-def pMorphism (M : Kripke.Model α) (M_trans : Transitive M.Frame) (r : M.World) : M.TransitiveTreeUnravelling r →ₚ M :=
-  Model.PseudoEpimorphism.mkAtomic (Frame.TransitiveTreeUnravelling.pMorphism M.Frame M_trans r) $ by aesop;
+def pMorphism (M : Kripke.Model) (M_trans : Transitive M.Rel) (r : M.World) : M.TransitiveTreeUnravelling r →ₚ M :=
+  Model.PseudoEpimorphism.mkAtomic (Frame.TransitiveTreeUnravelling.pMorphism M.toFrame M_trans r) $ by aesop;
+
+lemma modal_equivalence_at_root (M : Kripke.Model) (M_trans : Transitive M.Rel) (r : M.World)
+  : ModalEquivalent (M₁ := M.TransitiveTreeUnravelling r) (M₂ := M) ⟨[r], by simp⟩ r
+  := Model.PseudoEpimorphism.modal_equivalence (Model.TransitiveTreeUnravelling.pMorphism M M_trans r) (⟨[r], by simp⟩)
 
 end Model.TransitiveTreeUnravelling
 
@@ -198,11 +179,6 @@ structure FiniteTransitiveTree extends Kripke.FiniteFrame, Kripke.RootedFrame wh
   rel_assymetric : Assymetric Rel
   rel_transitive : Transitive Rel
 
-set_option linter.unusedVariables false in
-protected abbrev FiniteTransitiveTree.Dep (α : Type*) := FiniteTransitiveTree
-protected abbrev FiniteTransitiveTree.alt (T : FiniteTransitiveTree) {α} : FiniteTransitiveTree.Dep α := T
-postfix:max "#" => FiniteTransitiveTree.alt
-
 namespace FiniteTransitiveTree
 
 lemma rel_irreflexive (T : FiniteTransitiveTree) : Irreflexive T.Rel := irreflexive_of_assymetric $ T.rel_assymetric
@@ -210,38 +186,23 @@ lemma rel_irreflexive (T : FiniteTransitiveTree) : Irreflexive T.Rel := irreflex
 end FiniteTransitiveTree
 
 
-abbrev Model.FiniteTransitiveTreeUnravelling (M : Kripke.Model α) (r : M.World) : Kripke.Model α := (M↾r).TransitiveTreeUnravelling ⟨r, by tauto⟩
+abbrev Model.FiniteTransitiveTreeUnravelling (M : Kripke.Model) (r : M.World) : Kripke.Model := (M↾r).TransitiveTreeUnravelling ⟨r, by tauto⟩
 
-structure FiniteTransitiveTreeModel (α) where
-  Tree : FiniteTransitiveTree
-  Valuation : Valuation Tree.toFrame α
 
-namespace FiniteTransitiveTreeModel
-
-abbrev World (M : FiniteTransitiveTreeModel α) := M.Tree.World
-
-abbrev root (M : FiniteTransitiveTreeModel α) : M.World := M.Tree.root
-
-abbrev toFrame (M : FiniteTransitiveTreeModel α) : Kripke.Frame := M.Tree.toFrame
-
-abbrev toModel (M : FiniteTransitiveTreeModel α) : Kripke.Model α := ⟨M.toFrame, M.Valuation⟩
-instance : Coe (FiniteTransitiveTreeModel α) (Kripke.Model α) := ⟨toModel⟩
-instance : CoeSort (FiniteTransitiveTreeModel α) (Type u) := ⟨World⟩
-
-end FiniteTransitiveTreeModel
+structure FiniteTransitiveTreeModel extends FiniteTransitiveTree, Model where
 
 
 abbrev FiniteFrame.FiniteTransitiveTreeUnravelling
   (F : FiniteFrame) [DecidableEq F.World] (F_trans : Transitive F.toFrame) (F_irrefl : Irreflexive F.toFrame) (r : F.World) : FiniteTransitiveTree :=
-  letI T := (F↾r).TransitiveTreeUnravelling ⟨r, by tauto⟩
+  letI T := (F.toFrame↾r).TransitiveTreeUnravelling ⟨r, by tauto⟩
   {
     World := T.World
     Rel := T.Rel
     rel_transitive := Frame.TransitiveTreeUnravelling.rel_transitive
     rel_assymetric := Frame.TransitiveTreeUnravelling.rel_asymmetric
     root_rooted := Frame.TransitiveTreeUnravelling.rooted
-    World_finite := by
-      have := F.World_finite;
+    world_finite := by
+      have := F.world_finite;
       simp [Frame.TreeUnravelling];
       suffices h : Finite { x // List.Chain' (F.PointGenerated r).Rel x } by
         exact Finite.of_injective (β := { x // List.Chain' (F.PointGenerated r).Rel x })
@@ -249,4 +210,6 @@ abbrev FiniteFrame.FiniteTransitiveTreeUnravelling
       exact List.chains_finite (Frame.PointGenerated.rel_transitive F_trans) (Frame.PointGenerated.rel_irreflexive F_irrefl)
   }
 
-end LO.Kripke
+end Kripke
+
+end LO.Modal
