Foundation/Vorspiel/Chain.lean
@@ -1,0 +1,24 @@
+import Mathlib.Data.Fintype.Card
+import Mathlib.Data.Fintype.List
+
+namespace List
+
+variable {l l₁ l₂ : List α}
+variable {R : α → α → Prop}
+
+lemma Chain'.nodup_of_trans_irreflex (R_trans : Transitive R) (R_irrefl : Irreflexive R) (h_chain : l.Chain' R) : l.Nodup := by
+  by_contra hC;
+  replace ⟨d, hC⟩ := List.exists_duplicate_iff_not_nodup.mpr hC;
+  have := List.duplicate_iff_sublist.mp hC;
+  have := @List.Chain'.sublist α R [d, d] l ⟨by aesop⟩ h_chain this;
+  simp at this;
+  exact R_irrefl d this;
+
+instance finiteNodupList [DecidableEq α] [Finite α] : Finite { l : List α // l.Nodup } := @fintypeNodupList α _ (Fintype.ofFinite α) |>.finite
+
+lemma chains_finite [DecidableEq α] [Finite α] (R_trans : Transitive R) (R_irrefl : Irreflexive R) : Finite { l : List α // l.Chain' R } := by
+  apply @Finite.of_injective { l : List α // l.Chain' R } { l : List α // l.Nodup } _ ?f;
+  case f => intro ⟨l, hl⟩; refine ⟨l, List.Chain'.nodup_of_trans_irreflex R_trans R_irrefl hl⟩;
+  simp [Function.Injective];
+
+end List
